@prefix part: <http://www.ontologydesignpatterns.org/cp/owl/participation.owl#> .
@prefix planex: <http://www.ontologydesignpatterns.org/cp/owl/basicplanexecution.owl#> .
@prefix pwo: <http://purl.org/spar/pwo/> .
@prefix rdf: <http://www.w3.org/1999/02/22-rdf-syntax-ns#> .
@prefix rdfs: <http://www.w3.org/2000/01/rdf-schema#> .
@prefix sh: <http://www.w3.org/ns/shacl#> .
@prefix taskex: <http://www.ontologydesignpatterns.org/cp/owl/taskexecution.owl#> .
@prefix ti: <http://www.ontologydesignpatterns.org/cp/owl/timeinterval.owl#> .
@prefix tisit: <http://www.ontologydesignpatterns.org/cp/owl/timeindexedsituation.owl#> .

pwo:happened
  a rdf:Property ;
  rdfs:label "happened"@en ;
  rdfs:comment "It allows one to link an event to the interval when it happened."@en ;
  rdfs:domain part:Event ;
  rdfs:range ti:TimeInterval ;
.

pwo:involvesAction
  a rdf:Property ;
  rdfs:label "involves action"@en ;
  rdfs:comment "The property linking a particular execution of a workflow to an action."@en ;
  rdfs:domain pwo:WorkflowExecution ;
  rdfs:range pwo:Action ;
.

pwo:Action
  a rdfs:Class ;
  rdfs:label "action" ;
  rdfs:comment "An event with at least one agent that is participant in it and that is linked to a workflow execution and to a step of the related workflow description." ;
  rdfs:subClassOf part:Event , planex:Action , taskex:Action ;
.

pwo:WorkflowExecution
  a rdfs:Class ;
  rdfs:subClassOf planex:PlanExecution , tisit:TimeIndexedSituation ;
.

pwo:OneHappenedInterval
  a sh:NodeShape ;
  sh:targetSubjectsOf pwo:happened ;
  sh:property [
    sh:path pwo:happened ;
    sh:maxCount 1 ;
  ] ;
.
